---
title: "CS140-lecture-20210901"
# date: 2021-09-01T10:17:03-07:00
draft: false
bookToc: true
tags: ["proof", "asymptotic analysis"]
---

## A note on learning in this class

On different levels of learning

![image_2021-09-01-10-29-10](/notes/image_2021-09-01-10-29-10.png)

We will strive for about 60% of problems being level 3.

When working on a problem, there can be 3 outcomes
- could solve it
- could not solve it
- solved, but incorrect

If solved incorrectly, tracing back to the exact part that went wrong can be really beneficial.

## Methods of proof cont.

### An easy starting example

Suppose that {{<k>}} x > 3 {{</k>}}, is {{<k>}} x^2-2y > 5 {{</k>}}?

<blockquote class="book-hint info">
Note: 
Remember, this is a universal statement.
So it is asking whether that is true for all {{<k>}} x {{</k>}} and {{<k>}} y {{</k>}}.
</blockquote>

The first thing we can try to do is disprove the statement.
We need to come up with values that show that this statement is false.
Lets say we let {{<k>}} x=4 {{</k>}}, and {{<k>}} y=10 {{</k>}}, so

{{<k display>}}
\begin{aligned}
    4^2 - 2(10) &> 5 \\
    -4 &\not > 5
\end{aligned}
{{</k>}}

So, by counter example, it is not true for all {{<k>}} x {{</k>}} and {{<k>}} y {{</k>}} values.

### Example 2

Suppose that {{<k>}} a,b \in \mathbb{R}  {{</k>}}.
If {{<k>}} 0 < a < b {{</k>}}, then {{<k>}} a^2 < b^2 {{</k>}}.
We can let

{{<k display>}}
\begin{aligned}
    p &= 0 < a < b \\
    q &= a^2 < b^2
\end{aligned}
{{</k>}}

The question is saying that "if {{<k>}} p {{</k>}} then {{<k>}} q {{</k>}}."

We can start by trying to see if {{<k>}} p \to q {{</k>}} is true.
Lets start with {{<k>}} p {{</k>}}, and see if we can get to {{<k>}}  {{</k>}}

{{<k display>}}
\begin{aligned}
    0 < a &< b\\
    a \cdot a &< b \cdot a \\
    a^2 &< ab\\
\end{aligned}
{{</k>}}

Also,

{{<k display>}}
\begin{aligned}
    a \cdot b &< b \cdot b \\
    ab &< b^2
\end{aligned}
{{</k>}}

And we can plug it back in:

{{<k display>}}
\begin{aligned}
    a^2 < ab < b^2 \\
    a^2 < b^2
\end{aligned}
{{</k>}}

### Example 3

Suppose that {{<k>}} a,b,c \in \mathbb{R}  {{</k>}} and {{<k>}} a > b {{</k>}}.
If {{<k>}} ac \leq bc {{</k>}}, then {{<k>}} c \leq 0 {{</k>}}.

Looking at the direct method to solve this

{{<k display>}}
\begin{aligned}
    ac \leq bc \to c \leq 0
\end{aligned}
{{</k>}}

show that it may be difficult to prove that given the constraints above.
We can look at the opposite direction (remembering that {{<k>}} a > b {{</k>}}),

{{<k display>}}
\begin{aligned}
    c \leq 0 \to ac \leq bc
\end{aligned}
{{</k>}}

to see that the problem is more doable.

If {{<k>}} c = 0 {{</k>}}, then 

{{<k display>}}
\begin{aligned}
    ac = bc
\end{aligned}
{{</k>}}

and if {{<k>}} c < 0 {{</k>}}, then

{{<k display>}}
\begin{aligned}
    c( a > b) = ac \leq bc
\end{aligned}
{{</k>}}

So in this case it was easier to prove {{<k>}} \neg q \to \neg p {{</k>}}.

### Example 4

Show that for any natural number {{<k>}} n {{</k>}},

{{<k display>}}
\begin{aligned}
    2^0 + 2^1 + \cdots + 2^n = 2^{n+1} - 1
\end{aligned}
{{</k>}}

If we call this function {{<k>}} p(n) {{</k>}}, then the problem is really asking {{<k>}} \forall n \in \mathbb{N} : p(n) {{</k>}} (is true).
For this problem, we can try mathematical induction.

Since the domain for this is natural numbers, we can start from 0 and increase.
{{<k>}} p(0) {{</k>}} should be the base case, lets see:

{{<k display>}}
\begin{aligned}
    p(0) &= 2^0 = 2^{0+1} - 1 & \text{true}\\
\end{aligned}
{{</k>}}

The inductive step:
Suppose that {{<k>}} p(n) {{</k>}} is true, we show
that {{<k>}} p(n+1) {{</k>}} is true.

{{<k display>}}
\begin{aligned}
    p(n) &= 2^0 + 2^1 + \cdots + 2^n = 2^{n+1} - 1 \\
    p(n+1) &= 2^0 + 2^1 + \cdots + 2^{n+1} = 2^{(n+1)+1} - 1
\end{aligned}
{{</k>}}

Lets start with the left side of {{<k>}} p(n+1) {{</k>}}, and substitute in {{<k>}} p(n) {{</k>}}

{{<k display>}}
\begin{aligned}
    \overbrace{\underbrace{2^0 + 2^1 + \cdots + 2^n}_{p(n)} + 2^{n+1}}^{p(n+1)} &= (2^{n+1} - 1) + 2^{n+1} \\
    &= 2 \cdot 2^{n+1} - 1 \\
    &= 2^{(n+1)+1} - 1
\end{aligned}
{{</k>}}

So, by mathematical induction it is true.

### Example 5

Show that {{<k>}} \forall n \geq 5 : 2^n > n^2 {{</k>}}.

<blockquote class="book-hint info">
Note:
Since the variable is named {{<k>}} n {{</k>}}, and {{<k>}} n {{</k>}} starts as being equal to or greater than a natural number, we can assume
that {{<k>}} n {{</k>}} is also a natural number.
If {{<k>}} n {{</k>}} was real, the problem would most likely explicitly state
that {{<k>}} n {{</k>}} is real.
</blockquote>

Lets use mathematical induction for this problem, with the base case being {{<k>}} p(5) {{</k>}}:

{{<k display>}}
\begin{aligned}
    p(5) &= 2^5 > 5^2 \\
    &= 32 > 25 &\text{true}
\end{aligned}
{{</k>}}

Inductive step: Assume {{<k>}} p(n) {{</k>}} is true, show 
that {{<k>}} p(n+1) {{</k>}} is true,

{{<k display>}}
\begin{aligned}
    p(n) &= 2^n > n^2 \\
    p(n+1) &= 2^{n+1} > (n+1)^2
\end{aligned}
{{</k>}}

Lets start with the left side of {{<k>}} p(n+1) {{</k>}}, and substitute in {{<k>}} p(n) {{</k>}}

{{<k display>}}
\begin{aligned}
    2^{n+1} = 2 \cdot 2^n &> 2 \cdot n^2 = 2 n^2 \\
\end{aligned}
{{</k>}}

Lets see if we can make {{<k>}} 2n^2 {{</k>}} as similar to {{<k>}} (n+1)^2 {{</k>}} as possible

{{<k display>}}
\begin{aligned}
    2n^2 \geq n^2 + 2n + 1 \\
    n^2 \geq 2n + 1 \\
    n \geq 2 + \frac{1}{n}
\end{aligned}
{{</k>}}

So as long as 

{{<k display>}}
\begin{aligned}
    n \geq 2 + \frac{1}{5}
\end{aligned}
{{</k>}}

We can argue that since

{{<k display>}}
\begin{aligned}
    n \geq 2 + 1 \geq 2 + \frac{1}{n}
\end{aligned}
{{</k>}}

So,

{{<k display>}}
\begin{aligned}
    2^{n+1} \geq (n+1)^2
\end{aligned}
{{</k>}}

### Example 6

Show that for any {{<k>}} n > 0 {{</k>}}, a {{<k>}} 2^n \times 2^n {{</k>}} grid square with any one square removed can be covered with L shaped tiles.

![image_2021-09-01-12-08-39](/notes/image_2021-09-01-12-08-39.png)

So for {{<k>}} n = 1 {{</k>}}:

![image_2021-09-01-12-09-26](/notes/image_2021-09-01-12-09-26.png)
![image_2021-09-01-12-09-33](/notes/image_2021-09-01-12-09-33.png)

The domain of this problem is all the squares made up of {{<k>}} 2^n \times 2^n {{</k>}}, with the base case being {{<k>}} n = 1 {{</k>}}.
So we can use mathematical induction.

The base case for the {{<k>}} 2 \times 2 {{</k>}} grid shows
that if any of the squares are removed, the rest can be covered with an L shape.
We can show all 4 cases:

![image_2021-09-01-12-11-56](/notes/image_2021-09-01-12-11-56.png)

The inductive step: lets assume that it is true for {{<k>}} 2^n \times 2^n {{</k>}} grid sizes, lets show it is true for
{{<k>}} 2^{n+1} \times 2^{n+1} {{</k>}} grid sizes also.

If we think of one square being removed in the top right quadrant, we can cover that with an L shape.

![image_2021-09-01-12-14-41](/notes/image_2021-09-01-12-14-41.png)

Then we can think of that entire quadrant as being the square removed, and cover the middle 3 with an L shape.

![image_2021-09-01-12-16-37](/notes/image_2021-09-01-12-16-37.png)

The rest of each quadrant can now be covered with another L shape each.

## Asymptotic analysis

{{< hint info >}}
File: [*140-1.pdf*](/notes/140-1.pdf) 
{{< /hint >}}

![image_2021-09-01-15-14-26](/notes/image_2021-09-01-15-14-26.png)
![image_2021-09-01-15-14-54](/notes/image_2021-09-01-15-14-54.png)
![image_2021-09-01-15-16-24](/notes/image_2021-09-01-15-16-24.png)

Anything worse than polynomial time, generally is not practical.

If we double the input size in a polynomial-time function, the algorithm should only slow down by some constant factor, ie

{{<k display>}}
\begin{aligned}
    n^2 \to (2n)^2 \to 4n^2
\end{aligned}
{{</k>}}

Compare with a non-polynomial run time:

{{<k display>}}
\begin{aligned}
    2^n \to 2^{2n} \to 2^n \cdot 2^n
\end{aligned}
{{</k>}}

this shows that it does **not** increase by a constant factor, therefore it is not a polynomial time.

![image_2021-09-01-15-19-37](/notes/image_2021-09-01-15-19-37.png)

![image_2021-09-01-15-22-00](/notes/image_2021-09-01-15-22-00.png)

Execution time depends greatly on the hardware that the program is running on.

![image_2021-09-01-15-22-23](/notes/image_2021-09-01-15-22-23.png)

### Example 1

![image_2021-09-01-15-22-25](/notes/image_2021-09-01-15-22-25.png)

The total cost of algorithm 1 is {{<k>}} c_1 N {{</k>}}

The loop in algorithm 2 will run {{<k>}} N+1 {{</k>}} times, and the body of the loop will run {{<k>}} N {{</k>}} times, so the total cost is {{<k>}} (c_2 + c_1) N + c_2 {{</k>}}

![image_2021-09-01-15-24-40](/notes/image_2021-09-01-15-24-40.png)

The outer loop runs {{<k>}} N+1 {{</k>}} times, and the inner loop run {{<k>}} (N+1)N {{</k>}}.
The body of the inner loop will run {{<k>}} N \cdot N {{</k>}} times.
So, the total cost is

{{<k display>}}
\begin{aligned}
    c_1 + c_2(N+1) + c_2 N (N+1) + c_3 N^2
\end{aligned}
{{</k>}}

### Comparing algorithms

When analyzing an algorithm, we will go with a rough measure of the total cost.
This is usually the highest degree, the rate of growth, of the function.

![image_2021-09-01-15-28-09](/notes/image_2021-09-01-15-28-09.png)
![image_2021-09-01-15-30-25](/notes/image_2021-09-01-15-30-25.png)

The rate of growth is dominated by the cost of elephants because they cost a lot more. 
So the rate of growth can be approximated by just looking at the cost of elephants.

### Asymptotic notation

![image_2021-09-01-15-31-28](/notes/image_2021-09-01-15-31-28.png)

- Big {{<k>}} O {{</k>}}, upper bound
- Big {{<k>}} \Theta {{</k>}}, exact bound
- Big {{<k>}} \Omega {{</k>}}, lower bound

When looking for a tight bound, look for the Big {{<k>}} \Theta {{</k>}}.

![image_2021-09-01-15-35-10](/notes/image_2021-09-01-15-35-10.png)

If we have

{{<k display>}}
\begin{aligned}
    2n^2 - n + 5
\end{aligned}
{{</k>}}

the {{<k>}} n^2 {{</k>}} dominates as {{<k>}} n \to \infty {{</k>}}.
So the runtime is {{<k>}} O(n^2) {{</k>}}.

![image_2021-09-01-15-37-41](/notes/image_2021-09-01-15-37-41.png)

While the algorithms may start with {{<k>}} f_B {{</k>}} being faster, once {{<k>}} n {{</k>}} gets large enough it will grow faster than {{<k>}} f_A {{</k>}}.

![image_2021-09-01-15-38-49](/notes/image_2021-09-01-15-38-49.png)

<blockquote class="book-hint info">
Note: 
If we have

{{<k display>}}
\begin{aligned}
    2n^2 + 5 \lg n
\end{aligned}
{{</k>}}

the exponential term will **always** dominate the logarithmic term, so {{<k>}} O(n^2) {{</k>}}.
</blockquote>

![image_2021-09-01-15-43-55](/notes/image_2021-09-01-15-43-55.png)
![image_2021-09-01-15-44-29](/notes/image_2021-09-01-15-44-29.png)
![image_2021-09-01-15-45-56](/notes/image_2021-09-01-15-45-56.png)
![image_2021-09-01-15-47-51](/notes/image_2021-09-01-15-47-51.png)

### Example problems

Prove that {{<k>}} 2n^2 = O(n^3) {{</k>}}.

We want to find {{<k>}} c {{</k>}} and {{<k>}} n_0 {{</k>}} such
that {{<k>}} \forall n \geq n_0: 0 \leq f(n) \leq c(g(n)) {{</k>}}.

So, 

{{<k display>}}
\begin{aligned}
    2n^2 &\leq c n^3
\end{aligned}
{{</k>}}

and solve for {{<k>}} c {{</k>}}.

{{<k display>}}
\begin{aligned}
    2 &\leq cn \\
    \frac{2}{n} &\leq c
\end{aligned}
{{</k>}}

So this works when {{<k>}} c = 2 {{</k>}} and {{<k>}} n = 1 {{</k>}}, and up.
So our initial {{<k>}} n {{</k>}} value 
that works is {{<k>}} 1 {{</k>}}, so {{<k>}} n_0 = 1 {{</k>}}.
This makes the equality true for all values higher than the initial.

<blockquote class="book-hint info">
Note: The functions can cross each other, but after the value {{<k>}} n_0 {{</k>}}, the functions no longer cross.
</blockquote>

---

Prove that {{<k>}} n^2 = O(n^2) {{</k>}}.

{{<k display>}}
\begin{aligned}
    n^2 \leq cn^2 \to c \geq 1
\end{aligned}
{{</k>}}

So {{<k>}} c = 1 {{</k>}} and {{<k>}} n_0 = 1 {{</k>}}.

---

Prove that {{<k>}} 1000n^2 + 1000n = O(n^2) {{</k>}}.

{{<k display>}}
\begin{aligned}
    1000n^2 + 1000n \leq cn^2
\end{aligned}
{{</k>}}

This doesn't show an easy value for {{<k>}} c {{</k>}}.
So we can think of it as

{{<k display>}}
\begin{aligned}
    1000n^2 + 1000n &\leq 1000n^2 + 1000 n^2 \\
    &= 2000 n^2
\end{aligned}
{{</k>}}

This works when {{<k>}} n \geq 1 {{</k>}}.

So our {{<k>}} c = 2000 {{</k>}}, and {{<k>}} n_0 = 1 {{</k>}}.

<blockquote class="book-hint info">
Note: So the general idea here was to transform the {{<k>}} n {{</k>}} term so it can be combined, and it is easier to see
what the {{<k>}} c {{</k>}} value should be.
</blockquote>

---

Prove that {{<k>}} n = O(n^2) {{</k>}}.

{{<k display>}}
\begin{aligned}
    n &\leq cn^2 \\
    cn &\geq 1
\end{aligned}
{{</k>}}

So when {{<k>}} c = 1 {{</k>}} and {{<k>}} n_0 = 1 {{</k>}} it is true.

---

Show that {{<k>}} 30n + 8 {{</k>}} is {{<k>}} O(n) {{</k>}}.

{{<k display>}}
\begin{aligned}
    30n + 8 &\leq cn \\
    30n + 8 &\leq 30n + n \\
    30n + 8 &\leq 31n
\end{aligned}
{{</k>}}

Note that this is only true when {{<k>}} n > 8 {{</k>}}, so our values are {{<k>}} c = 31 {{</k>}} and {{<k>}} n_0 = 8 {{</k>}}.

![image_2021-09-01-16-21-46](/notes/image_2021-09-01-16-21-46.png)

The point where they cross is {{<k>}} n_0 {{</k>}}.

### No uniqueness

![image_2021-09-01-16-22-30](/notes/image_2021-09-01-16-22-30.png)

### Trying to prove something that is not true

Lets try to prove {{<k>}} 4n^2 = O(n) {{</k>}}.

{{<k display>}}
\begin{aligned}
    4n^2 &\leq cn \\
    4n &\leq c
\end{aligned}
{{</k>}}

Since {{<k>}} n {{</k>}} does not have an upper bound, we cannot have our constant {{<k>}} c {{</k>}} always larger than an arbitrarily large {{<k>}} n {{</k>}}.
This is a contradiction.

---

Show that {{<k>}} n^2 - 2n + 3 \lg n = O(n^2) {{</k>}}.

{{<k display>}}
\begin{aligned}
    n^2 - 2n + 3 \lg n &\leq cn^2 \\
    &\leq n^2 + 3 \lg n \\
    &\leq n^2 + 3n
\end{aligned}
{{</k>}}

Which we can do because

{{<k display>}}
\begin{aligned}
    \lg n \leq n \\
    n \leq 2^n
\end{aligned}
{{</k>}}

So {{<k>}} n_0 = 1 {{</k>}}, and we can see this is true by {{<k>}} 1 \leq 2^1 = 2 {{</k>}}.
The terms can combine to get {{<k>}} c = 4 {{</k>}}:

{{<k display>}}
\begin{aligned}
    &\leq n^2 + 3 n^2 \\
    &\leq 4n^2
\end{aligned}
{{</k>}}

